wip

proof/correctness/Correctness_Address.ec
@@ -4,12 +4,17 @@ require import AllCore List Distr RealExp IntDiv.
 
 from Jasmin require import JModel.
 
-require import Array8 Array32.
+require import BitEncoding.
+(*---*) import BitChunking.
 
-require import Address.
+require import Array4 Array8 Array32.
+require import WArray4.
+
+require import Params Address.
 require import XMSS_IMPL.
 
 op zero_addr : adrs = Array8.init (fun _ => W32.zero). 
+op W32toBytes (x : W32.t) : W8.t list = map W8.bits2w (chunk W8.size (W32.w2bits x)).
 
 lemma zero_addr_op_impl (address : adrs) :
     hoare[M(Syscall)._zero_address : true ==> res = zero_addr].
@@ -37,21 +42,88 @@ lemma zero_addr_res (address : adrs) :
     phoare[M(Syscall)._zero_address : true ==> res = zero_addr] = 1%r
       by conseq zero_addr_ll (zero_addr_op_impl address) => //=. 
 
-lemma _addr_to_bytes_correctness (x : W32.t Array8.t) : 
-    hoare[M(Syscall).__addr_to_bytes : 
-        arg.`2 = x ==> to_list res = addr_to_bytes x].
+import W4u8.Pack.
+
+lemma u32_to_bytes_correct (x : W32.t) :
+    hoare [M(Syscall).__u32_to_bytes : arg.`2 = x ==> to_list res = W32toBytes x].
 proof.
 proc.
-admit. 
+auto => /> &hr.
+rewrite /W32toBytes.
+apply (eq_from_nth witness).
+  + rewrite size_to_list size_map size_chunk //. 
+rewrite size_to_list => i?. 
+rewrite get_to_list initiE // (nth_map witness).
+  + rewrite size_chunk //. 
+rewrite /BSWAP_32 => />.
+rewrite ifT // /chunk nth_mkseq /(\bits8) => />.
+rewrite wordP => j?.
+rewrite initiE // /(\o) => />. 
+rewrite /bits2w => />.
+rewrite initiE // nth_take // 1:/# nth_drop 1,2:/# /w2bits nth_mkseq 1:/# => />.
+rewrite /unpack8 => />.
+admit.
+qed.
+
+(*****) import StdBigop.Bigint.
+
+lemma _addr_to_bytes_correctness (x : W32.t Array8.t) : 
+    n = 32 =>
+    hoare[M(Syscall).__addr_to_bytes : 
+        arg.`2 = x ==> to_list res = val (addr_to_bytes x)].
+proof.
+move => n_val.
+proc.
+while (
+  #pre /\
+  0 <= i <= 8 /\
+  forall (k : int), 0 <= k < 4*i => addr_as_bytes.[k] = nth witness (val (addr_to_bytes x)) k
+).
+    + seq 2 : (#pre /\ to_list buf = W32toBytes addr.[i]).
+         * ecall (u32_to_bytes_correct addr.[i]); auto => />. 
+      auto => /> &hr H0 H1 H2 H3 H4. 
+      do split; 1,2: by smt(). 
+      move => k??.
+      rewrite initiE 1:/# => />. 
+      case (4 * i{hr} <= k < 4 * i{hr} + 4) => *.
+         * rewrite -get_to_list H4 /W32toBytes /addr_to_bytes.
+           rewrite (nth_map witness); [rewrite size_chunk // size_w2bits /# |] => />.
+           rewrite insubdK.  
+              - rewrite /P /BitsToBytes size_map size_chunk // size_flatten sumzE BIA.big_map /(\o) //=. 
+                rewrite -(StdBigop.Bigint.BIA.eq_big_seq (fun _ => 32)) /=. 
+                      + admit.
+                rewrite big_constz count_predT size_mkseq n_val /#.
+           rewrite /BitsToBytes. 
+           rewrite (nth_map witness); [rewrite size_iota size_w2bits /# |].
+           rewrite size_w2bits nth_iota 1:/# => />.
+           rewrite wordP => j?.
+           rewrite (nth_map witness). 
+              - rewrite size_chunk // size_flatten sumzE BIA.big_map /(\o) //=. 
+                rewrite -(StdBigop.Bigint.BIA.eq_big_seq (fun _ => 32)).
+                      + admit.
+                rewrite big_constz count_predT size_mkseq /#.
+           rewrite /chunk nth_mkseq => />.
+              - admit.
+           rewrite /w2bits.
+           admit.
+         * rewrite H2 // /#.
+    + auto => /> &hr.
+      split => [/# |].
+      move => addBytes j ???.
+      have ->: j = 8 by smt(). 
+      move => H.
+      apply (eq_from_nth witness).
+         * rewrite size_to_list valP n_val //.
+      rewrite size_to_list => k?. 
+      rewrite get_to_list H //. 
 qed.
 
 lemma addr_to_bytes_ll : islossless M(Syscall).__addr_to_bytes by proc; inline; while (true) (8 - i); auto => /> /#.
 
 lemma addr_to_bytes_correctness (x : W32.t Array8.t) : 
     phoare[M(Syscall).__addr_to_bytes : arg.`2 = x ==> 
-      to_list res = addr_to_bytes x] = 1%r.
+      to_list res = val (addr_to_bytes x)] = 1%r.
 proof.
 proc.
-(* conseq addr_to_bytes_ll (_addr_to_bytes_correctness x). *)
 admit.
 qed.
