proof/correctness/Correctness_Bytes.ec
@@ -5,7 +5,7 @@ from Jasmin require import JModel.
 
 require import XMSS_IMPL.
 
-require import Array32.
+require import Array2 Array32.
 
 require import Hash.
 require import Termination.
@@ -27,7 +27,6 @@ lemma ull_to_bytes_32_correct (x : W64.t) :
 (** -------------------------------------------------------------------------------------------- **)
 
 
-
 (*
 lemma ull_to_bytes_2_correct (y : W64.t) :
     hoare [M(Syscall).__ull_to_bytes_2 : 
@@ -46,5 +45,4 @@ lemma ull_to_bytes_2_equiv (y : W64.t) :
       arg.`2 = y ==> 
         to_list res = toByte (W32.of_int (to_uint y)) 2] = 1%r
           by conseq ull_to_bytes_2_ll (ull_to_bytes_2_correct y) => //.
-
 *)
