proof/correctness/Correctness_Mem.ec
@@ -9,6 +9,90 @@ require import XMSS_IMPL.
 require import Utils2. (* valid_ptr predicate *)
 require import Termination.
 
+lemma _memcpy_u8u8_2_32_2144_post (_in : W8.t Array2144.t, oi :W64.t):
+    hoare [
+      M(Syscall).__memcpy_u8u8_2_32_2144 : 
+      arg.`2 = _in /\
+      arg.`3 = oi /\
+      arg.`4 = W64.of_int 32 /\
+      0 <= to_uint oi < W32.max_uint /\
+      0 <= to_uint (oi + W64.of_int 32) < 2144
+      ==>
+      to_list res.`1 = sub _in (to_uint oi) 32
+    ].
+proof.
+proc => //=.
+while ( 
+  in_0 = _in /\ 
+  bytes = (of_int 32)%W64 /\
+  (0 <= to_uint oi < 2144) /\
+
+  0 <= to_uint i <= 32 /\
+  forall (k : int), 0 <= k < to_uint i => out.[k] = in_0.[to_uint in_offset + k]
+).
+    + auto => /> &hr H0 H1 H2 H3 H4 H5.  
+      do split; 1,2: smt(@W64). 
+      move => k??.
+      rewrite get_setE 1:#smt:(@W64).
+      case (k = to_uint i{hr}) => *. 
+      admit.
+      admit. 
+    + auto => /> &hr ????.
+      admit.
+qed.
+
+lemma memcpy_u8u8_2_32_2144_post (_in : W8.t Array2144.t, oi :W64.t):
+    phoare [
+      M(Syscall).__memcpy_u8u8_2_32_2144 : 
+      arg.`2 = _in /\
+      arg.`3 = oi /\
+      arg.`4 = W64.of_int 32 /\
+      0 <= to_uint oi < W32.max_uint /\
+      0 <= to_uint (oi + W64.of_int 32) < 2144
+      ==>
+      to_list res.`1 = sub _in (to_uint oi) 32
+    ] = 1%r.
+proof.
+admit.
+qed.
+
+lemma memcpy_u8u8_2_64_2144_post (_in : W8.t Array2144.t, oi : W64.t):
+    phoare [
+      M(Syscall).__memcpy_u8u8_2_64_2144 : 
+      arg.`2 = _in /\
+      arg.`3 = oi /\
+      arg.`4 = W64.of_int 64 /\
+      0 <= to_uint oi < W32.max_uint /\
+      0 <= to_uint (oi + W64.of_int 64) < 2144
+      ==>
+      to_list res.`1 = sub _in (to_uint oi) 64
+    ] = 1%r.
+proof.
+admit.
+qed.
+
+
+(** -------------------------------------------------------------------------------------------- **)
+
+lemma or_zero(w0 w1 : W8.t) : 
+    (w0 `|` w1 = W8.zero) <=> (w0 = W8.zero /\ w1 = W8.zero).
+proof.
+split; last first.
+  + move => [-> ->].
+    by rewrite or0w.
+  + rewrite !wordP => H.
+    case (w0 = W8.zero).
+      * move => -> /= k kb. move : (H k kb) => /= /#. 
+      * move => *. have Hk : exists k, 0 <= k < 8 /\ w0.[k]. 
+         - move : (W8.wordP w0 W8.zero); smt(W8.zerowE W8.get_out).
+        elim Hk => k [kb kval]. move : (H k kb). by rewrite orwE kval.
+qed.
+
+lemma xor_eq (w0 w1 : W8.t) :
+    w0 `^` w1 = W8.zero => w0 = w1 by smt(@W8). 
+    
+(** -------------------------------------------------------------------------------------------- **)
+
 (******************************************************************************)
 (******************               MEMSET                          *************)
 (******************************************************************************)
@@ -117,21 +201,6 @@ lemma memset_nseq :
        to_list res = nseq 4 W8.zero] = 1%r
           by conseq memset_zero_ll _memset_nseq; auto.
 
-lemma load_store  (mem : global_mem_t) (ptr : W64.t) (v : W8.t) :
-    loadW8 (storeW8 mem (to_uint ptr) v) (to_uint ptr) = v 
-      by rewrite /storeW8 /loadW8 get_setE ifT.
-
-
-
-
-
-
-
-
-
-
-
-
 lemma memset_ptr_post (ptr : W64.t, len : W64.t, v : W8.t) :
     hoare [M(Syscall).__memset_u8_ptr : 
       0 <= to_uint len < W64.modulus /\
@@ -165,7 +234,6 @@ while (
          admit.
 qed.
 
-
 (******************************************************************************)
 (******************               MEMCPY                          *************)
 (******************************************************************************)
@@ -180,13 +248,28 @@ proof.
 proc.
 inline * ; wp ; sp.
 while (
+  in_ptr1  = ptr /\
+  0 <= (to_uint ptr) + 32 <= W64.modulus /\
+  0 <= to_uint ptr /\
+  
   0 <= i <= 32 /\
   0 <= to_uint in_ptr{hr} + 32 <= W64.modulus /\
   forall (k : int), 0 <= k < i => (out1.[k] = loadW8 Glob.mem ((to_uint ptr) + k))
-) ; auto => />; last first.
-- move => &hr *. split ; 1:smt(@JMemory). move => *. rewrite tP ; smt(@JMemory @Array32).
-- move => &hr *. split ; 1:smt(). move => k *. rewrite get_setE 1:/#. case (k = i{hr}); last by smt(@JMemory).
-  move => E0 ; congr. rewrite E0 to_uintD of_uintK //=. admit. (* overflow *)
+).
+    + auto => /> &hr H0 H1 H2 H3 H4 H5 H6 H7 H8C.
+      do split; 1,2:smt().
+      move => k??.
+      rewrite get_setE //=.
+      case (k = i{hr}) => E.
+          * congr; rewrite E #smt:(@W64 pow2_64).
+          * apply H7 => /#.      
+    + auto => /> &hr H0 H1 H2. 
+      split => [/# | i0 out0 ???]. 
+      have ->: i0 = 32 by smt().
+      move => H3.
+      rewrite tP => j?.
+      rewrite initiE //=. 
+      by apply H3.
 qed.
 
 lemma memcpy_ptr_ll :
@@ -213,38 +296,59 @@ proof.
 by conseq memcpy_ptr_ll (memcpy_ptr_correct ptr).
 qed.
 
-lemma _x_memcpy_u8u8_post (x : W8.t Array32.t) :
-    phoare [M(Syscall)._x_memcpy_u8u8_32_32 : arg.`2 = x ==> res = x] = 1%r.
+lemma _x_memcpy_u8u8_p (x : W8.t Array32.t) :
+hoare [M(Syscall)._x_memcpy_u8u8_32_32 : arg.`2 = x ==> res = x].
 proof.
-proc ; inline*.
-wp ; sp.
-while (* while invariante variante *)
-(0 <= to_uint i <= 32 /\ (forall (k : int), 0 <= k < to_uint i => (out1.[k] = in_01.[k]))) 
-(32 - to_uint i).
-  + auto => /> &hr i *; do split.
-      - smt(@W64).
-      - smt(@W64 pow2_64).
-      - move => k *. rewrite get_setE; 1:smt(@W64). case (k = to_uint i{hr}).
-           * move => * /#. 
-           * move => *. admit.
-      - smt(@W64 pow2_64).
-  + skip => /> &hr *. split; 1:smt(). progress.
-      - smt(@W64).
-      - rewrite tP. smt.
+proc.
+inline.
+wp; sp.
+while (
+  0 <= to_uint i <= 32 /\ 
+  (forall (k : int), 0 <= k < to_uint i => (out1.[k] = in_01.[k])) /\
+
+  in_01 = x
+).
+    + auto => /> &hr H0 H1 H2 H3. 
+      do split; 1,2: by smt(@W64).
+      move => k??.
+      rewrite get_setE 1:#smt:(@W64).
+      case (k = to_uint i{hr}) => [/# | *].
+      apply H2.
+      smt(@W64).
+    + skip => /> &hr.
+      split => [/# | i0 out10 ???].
+      have ->: to_uint i0 = 32 by smt(@W64 pow2_64).
+      by rewrite tP.
 qed.
+
+
+lemma _x_memcpy_u8u8_post (x : W8.t Array32.t) :
+    phoare [
+        M(Syscall)._x_memcpy_u8u8_32_32 : 
+          arg.`2 = x ==> res = x] = 1%r
+            by conseq _x_memcpy_u8u8_32_32_ll (_x_memcpy_u8u8_p x).
 
 lemma _x_memcpy_u8u8_64_ (x : W8.t Array64.t) :
     hoare [M(Syscall)._x_memcpy_u8u8_64_64 : arg.`2 = x ==> res = x].
 proof.
-proc => //=. 
+proc. 
 inline; wp; sp. 
 while (
   in_01 = x /\
   0 <= to_uint i <= 64 /\
   (forall (k : int), 0 <= k < to_uint i => (out1.[k] = x.[k]))
 ).
-    + auto => /> &hr *; do split; 1,2:smt(@W64); move => k *. rewrite get_setE; first by smt(@W64). admit. (* case (k = to_uint i{hr}) ; first by smt(). *)
-    + auto => /> &hr; split; [ smt() | move => *; rewrite tP; smt(@W64 pow2_64) ].
+    + auto => /> &hr H0 H1 H2 H3.
+      do split; 1,2: by smt(@W64). 
+      move => k??. 
+      rewrite get_setE 1:#smt:(@W64).
+      case (k = to_uint i{hr}) => [/# | *].
+      apply H2.
+      smt(@W64).
+    + auto => /> &hr.
+      split => [/# | i0 out10 ???].
+      have ->: to_uint i0 = 64 by smt(@W64 pow2_64).
+      by rewrite tP.
 qed.
 
 
@@ -262,43 +366,40 @@ lemma memcmp_true (x y : W8.t Array32.t) :
         hoare[M(Syscall).__memcmp : arg = (x, y) ==> res = W8.zero].
 proof.
 move => xy_eq.
-proc ; auto => /> *.
+proc.
 while(0 <= to_uint i <= 32 /\ a = b /\ acc = W8.zero) ; auto => /> *; smt(@W64).
-qed.
-
-lemma or_zero(w0 w1 : W8.t) : 
-    (w0 `|` w1 = W8.zero) <=> (w0 = W8.zero /\ w1 = W8.zero).
-proof.
-split; last first.
-  + move => [-> ->].
-    by rewrite or0w.
-  + rewrite !wordP => H.
-    case (w0 = W8.zero).
-      * move => -> /= k kb. move : (H k kb) => /= /#. 
-      * move => *. have Hk : exists k, 0 <= k < 8 /\ w0.[k]. 
-         - move : (W8.wordP w0 W8.zero); smt(W8.zerowE W8.get_out).
-        elim Hk => k [kb kval]. move : (H k kb). by rewrite orwE kval.
 qed.
 
 lemma memcmp_false (x y : W8.t Array32.t) :
     x <> y => 
         hoare[M(Syscall).__memcmp : arg = (x, y) ==> res <> W8.zero].
 proof.
-move => xy_neq.
+move => ?. 
+have E : exists (i : int), 0 <= i < 32 => x.[i] <> y.[i] by smt(@Array32). 
 proc.
-auto => />.
-have E0 : exists (z : int), 0 <= z < 32 => x.[z] <> y.[z] by smt(@Array67).
 while (
   #pre /\
+  (exists (i : int), 0 <= i && i < 32 => x.[i] <> y.[i]) /\
   0 <= to_uint i <= 32 /\ 
-  (exists (k : int), 0 <= k < to_uint i => (a.[k] = b.[k]) => acc <> W8.zero)
-); last first.
-    + auto => />. split; 1:smt(). move => acc i. rewrite /(\ult) of_uintK => ???.
-      have -> : to_uint i = 32 by smt(@W64 pow2_64). move => k ?. admit.
-
-    + auto => /> &r. rewrite !/(\ult) !to_uintD !of_uintK //=. progress;1,2:smt(@W64 pow2_64).
-admit.
+  (acc = W8.zero <=> forall (k : int), 0 <= k < to_uint i => x.[k] = y.[k])
+). 
+    + auto => /> &hr i0???H0. 
+      rewrite ultE of_uintK (: 32 %% W64.modulus = 32) 1:/# => ?. 
+      do split; 1,2: smt(@W64).       
+         * move => H. 
+           have E1 : acc{hr} = W8.zero by smt(or_zero). 
+           have E2 : x.[to_uint i{hr}] `^` y.[to_uint i{hr}] = W8.zero by smt(or_zero).
+           have E3 : x.[to_uint i{hr}] = y.[to_uint i{hr}] by smt(xor_eq).
+           have E4 : forall (k : int), 0 <= k && k < to_uint i{hr} => x.[k] = y.[k] by smt(). 
+           rewrite to_uintD_small /#.
+         * rewrite to_uintD_small 1:/# (: to_uint W64.one = 1) 1:/# => H.
+           rewrite or_zero; split; [rewrite H0 | rewrite H ] => /#.
+    + auto => />; split => [/# | acc0 i0]. 
+      rewrite ultE -lezNgt of_uintK //= => [?i1??? ->].
+      have ->: to_uint i0 = 32 by smt(). 
+      smt(@Array32). 
 qed.
+
 
 (* INLEN = 32 /\ OUTLEN = 2144 *)
 (* pre: copying all elements of in does not write out of bounds in out *)
@@ -306,9 +407,14 @@ qed.
 (* 0 <= offset <= 2112 *)
 (* same as memcpy(out + offset, in, sizeof(in)); *)
 lemma memcpy_offset_1 (_out_ : W8.t Array2144.t, _offset_ : W64.t, _in_ : W8.t Array32.t) :
-    hoare [M(Syscall).__memcpy_u8u8_offset : 
-      arg.`2=_offset_ /\ arg.`3=_in_ /\  0 <= to_uint _offset_ <= 2122 ==>
-        (forall (k : int), 0 <= k < 32 => (res.[to_uint _offset_ + k] = _in_.[k]))].
+    hoare [
+      M(Syscall).__memcpy_u8u8_offset : 
+      arg.`2=_offset_ /\ 
+      arg.`3=_in_ /\  
+      0 <= to_uint _offset_ <= 2122 
+      ==>
+      (forall (k : int), 0 <= k < 32 => (res.[to_uint _offset_ + k] = _in_.[k]))
+    ].
 proof.
 proc.
 sp.
@@ -328,3 +434,36 @@ while (
     + move => ???. rewrite get_setE. split ; 1:smt(). move => ?. admit. admit.
 qed.
 
+lemma nbytes_copy_inplace_correct (x : W8.t Array2144.t, oo oi : W64.t) :
+    hoare [
+      M(Syscall).__nbytes_copy_inplace_2144 :
+      arg=(x, oo, oi) /\
+      0 <= to_uint oo /\
+      to_uint oo + 32 < 2144 /\
+      0 <= to_uint oi /\
+      to_uint oi + 32 < 2144
+      ==>
+      (forall (k : int), 0 <= k < 32 => res.[to_uint oo + k] = x.[to_uint oi + k]) /\ (* changed regions *)
+      (* values outside the range offset_out to offset_out + n - 1 remain unchanged *)
+      (forall (k : int), 0 <= k < 2144 => 
+          (k < to_uint oo \/ to_uint oo + 32 <= k) =>
+             res.[k] = x.[k])
+
+    ].
+proof.
+proc.
+while (
+  #pre /\
+  0 <= i <= 32 /\
+  (forall (k : int), 0 <= k < i => out.[to_uint offset_out + k] = out.[to_uint offset_in + k])
+); last by auto => /> /#.  
+auto => /> &hr H0 H1 H2 H3 H4 H5 H6 H7. 
+do split; 2,3: by smt().
+    + rewrite tP => j?. 
+      (* rewrite get_setE. *)
+      admit. 
+    + move => k??. 
+      rewrite get_setE; [rewrite to_uintD_small of_uintK #smt:(modz_small) |].
+      rewrite get_setE; [rewrite to_uintD_small of_uintK #smt:(modz_small) |].
+      admit. 
+qed.
